bedrock2: hardcode cases for access_size

bedrock2/src/BasicC64Semantics.v
@@ -1,9 +1,23 @@
 Require Import Coq.NArith.BinNatDef.
-Require Import bedrock2.BasicC64Syntax bedrock2.Semantics.
+Require Import bedrock2.Syntax bedrock2.BasicC64Syntax bedrock2.Semantics.
 Require bedrock2.String bedrock2.Map.SortedList bedrock2.Map.SortedListString.
-Require Import coqutil.Word.Interface. Require coqutil.Word.Naive.
+Require Import coqutil.Word.Interface coqutil.Datatypes.HList coqutil.Datatypes.PrimitivePair.
+Require coqutil.Word.Naive.
 Import ZArith.
-
+Definition word := Word.Naive.word 64 (proj2 (Zlt_is_lt_bool 0 64) eq_refl).
+Definition byte := Word.Naive.word 8 (proj2 (Zlt_is_lt_bool 0 8) eq_refl).
+Definition bytes_per sz := match sz with access_size.one => 1 | access_size.two => 2 | access_size.four => 4 | access_size.word => 8 end.
+Fixpoint combine (n : nat) : forall (bs : tuple byte n), word :=
+  match n with
+  | O => fun _ => word.of_Z 0
+  | S n => fun bs => word.or (word.of_Z (word.unsigned (pair._1 bs)))
+                             (word.slu (combine n (pair._2 bs)) (word.of_Z 8))
+  end.
+Fixpoint split (n : nat) (w :word) : tuple byte n :=
+  match n with
+  | O => tt
+  | S n => pair.mk (word.of_Z (word.unsigned w)) (split n (word.slu w (word.of_Z 8)))
+  end.
 Instance parameters : parameters :=
   let word := Word.Naive.word 64 (proj2 (Zlt_is_lt_bool 0 64) eq_refl) in
   let byte := Word.Naive.word 8 (proj2 (Zlt_is_lt_bool 0 8) eq_refl) in
@@ -30,10 +44,11 @@ Instance parameters : parameters :=
     | bopname.eq => fun a b => if word.eqb a b then word.of_Z 1 else word.of_Z 0
     end;
   (* TODO: bedrock2.Byte, bedrock2.Word8 *)
-  byte := byte;
+  Semantics.byte := byte;
   mem := SortedList.map (SortedList.parameters.Build_parameters word byte word.eqb word.ltu);
-  combine _ b w := word.or (word.slu w (word.of_Z 8)) (word.of_Z (word.unsigned b));
-  split _ w := (word.of_Z (word.unsigned w), word.slu w (word.of_Z 8));
+  Semantics.bytes_per := bytes_per;
+  Semantics.combine sz := combine (bytes_per sz);
+  Semantics.split sz := split (bytes_per sz);
   locals := SortedListString.map _;
   funname_eqb := String.eqb;
 |}.
